Uart semantics and proofs (cont'd) (#888)
* Finish BitfieldProperties by adding spec of write functions

Specification & proofs has been added for the following functions:
- bitfield_field32_write
- bitfield_bit32_write

The postcondition just states that the return value is basically what is
computed in the function body, which might be not very useful for its
callers. We will add or modify the postcondition later if needed.

* Finish spec_of_uart_putchar with while loops

* Revert IncrementWait Changes

* Remove Axioms and add comments

* Pull out status_matches_state s' val = true from read_step

* Sam's comments

firmware/Uart/UartSemantics.v
@@ -20,8 +20,11 @@ Local Open Scope string_scope. Local Open Scope Z_scope. Local Open Scope list_s
 
 (* Circuit specification *)
 Class circuit_behavior :=
-  { ncycles_processing : nat
-  }.
+  {
+    fifo_depth: nat;
+    ncycles_processing : nat
+  }
+  .
 
 Section WithParameters.
   Context {word: word.word 32} {mem: map.map word Byte.byte}
@@ -97,32 +100,31 @@ Section WithParameters.
        && is_flag_set status UART_STATUS_TXEMPTY_BIT
        && is_flag_set status UART_STATUS_TXIDLE_BIT
     | BUSY t =>
-      if Nat.eqb t 0 then
+      negb (is_flag_set status UART_STATUS_TXIDLE_BIT) &&
+      (if Nat.eqb t 0 then
         (* FIFO is empty *)
         is_flag_set status UART_STATUS_TXEMPTY_BIT &&
-        negb (is_flag_set status UART_STATUS_TXFULL_BIT) &&
-        negb (is_flag_set status UART_STATUS_TXIDLE_BIT)
-      else if Nat.ltb t 32 then
-        negb (is_flag_set status UART_STATUS_TXFULL_BIT) &&
-        negb (is_flag_set status UART_STATUS_TXEMPTY_BIT) &&
-        negb (is_flag_set status UART_STATUS_TXIDLE_BIT)
+        negb (is_flag_set status UART_STATUS_TXFULL_BIT)
       else
-        (* FIFO is full *)
         negb (is_flag_set status UART_STATUS_TXEMPTY_BIT) &&
-        is_flag_set status UART_STATUS_TXFULL_BIT &&
-        negb (is_flag_set status UART_STATUS_TXIDLE_BIT)
+        (if Nat.ltb t (fifo_depth * ncycles_processing)  then
+          negb (is_flag_set status UART_STATUS_TXFULL_BIT)
+        else
+          (* FIFO is full *)
+          is_flag_set status UART_STATUS_TXFULL_BIT))
     end.
 
   Definition read_step
     (s : state) (r : Register) (val : word) (s' : state) : Prop :=
     match r with
     | STATUS =>
+        status_matches_state s' val = true /\
         match s with
-        | IDLE => status_matches_state s val = true /\ s' = IDLE
-        | BUSY O =>
-            (status_matches_state s val = true /\ s' = IDLE)
-        | BUSY txlvl =>
-            (status_matches_state s val = true /\ s' = BUSY (txlvl - 1))
+        | IDLE => s' = IDLE
+        | BUSY n =>
+            (* tx can non-deterministically finish sending *)
+            (s' = IDLE)
+            \/ (exists n', n = S n' /\ s' = BUSY n')
         end
     | _ => False (* cannot read any other regs *)
     end.
@@ -132,9 +134,14 @@ Section WithParameters.
     match r with
     | WDATA =>
         match s with
-        | IDLE => s' = BUSY 1
+        | IDLE => s' = BUSY (ncycles_processing)
             (* writing to 4-byte WDATA reg fills the FIFO with the last byte *)
-        | BUSY tx => if Nat.leb tx 32 then s' = BUSY (tx + 1) else False
+        | BUSY tx => if Nat.leb tx (fifo_depth * ncycles_processing)
+            (* the maximum tx will be (fifo_depth + 1) * ncycles_processing
+               and the FIFO status will be full *)
+            then s' = BUSY (tx + (ncycles_processing))
+            (* if FIFO is full, you can't send more data *)
+          else False
         end
     | INTR_ENABLE => s' = s
     | INTR_TEST => s' = s
