firmware/Uart/UartProperties.v
@@ -45,6 +45,7 @@ Ltac normalize_body_of_function f ::= Tactics.rdelta.rdelta f.
 Section Proofs.
   Context {word: word.word 32} {mem: map.map word Byte.byte}
           {word_ok: word.ok word} {mem_ok: map.ok mem}.
+  Context {circuit_spec : circuit_behavior}.
 
   (* Plug in the right state machine parameters; typeclass inference struggles here *)
   Local Notation execution := (execution (M:=uart_state_machine)).
@@ -57,7 +58,6 @@ Section Proofs.
          constants [Properties.word_cst]).
 
   Ltac solve_status_valid :=
-    eexists; ssplit; try reflexivity;
       cbv [is_flag_set]; boolsimpl;
       repeat lazymatch goal with
              | |- (_ && _)%bool = true => apply Bool.andb_true_iff; split
@@ -74,24 +74,38 @@ Section Proofs.
       simpl;
       lia.
 
+  Ltac separate_flags :=
+    repeat lazymatch goal with
+           | H: (_ && _)%bool = true |- _ =>
+               apply andb_prop in H; logical_simplify
+           end.
+
+
   Lemma status_read_always_ok s :
     exists val s', read_step s STATUS val s'.
   Proof.
-    destruct s; unfold read_step; cbn [read_step status_matches_state].
-    { exists (word.or (word.slu (word.of_Z 1) (word.of_Z UART_STATUS_TXEMPTY_BIT))
+    destruct s; unfold read_step; cbn [read_step];
+    cbv [status_matches_state].
+    { (* s = IDLE => s' = IDLE *)
+      exists (word.or (word.slu (word.of_Z 1) (word.of_Z UART_STATUS_TXEMPTY_BIT))
                       (word.slu (word.of_Z 1) (word.of_Z UART_STATUS_TXIDLE_BIT))).
-      solve_status_valid.
+      exists IDLE.
+      split; [ solve_status_valid | reflexivity ].
     }
-    { destruct (Nat.eqb txlvl 0)%bool eqn:H.
-      { apply Nat.eqb_eq in H. subst.
-        exists (word.slu (word.of_Z 1) (word.of_Z UART_STATUS_TXEMPTY_BIT)).
-        solve_status_valid. }
-      { destruct txlvl; [discriminate | ].
-        destruct (Nat.ltb (S txlvl) 32)%bool eqn:Hl.
-        { exists (word.of_Z 0).
-          solve_status_valid. }
-        { exists (word.slu (word.of_Z 1) (word.of_Z UART_STATUS_TXFULL_BIT)).
-          solve_status_valid. }
+    { (* s = BUSY n *)
+      destruct (Nat.eqb txlvl 0)%bool eqn:H.
+      { (* s = BUSY O => s' = IDLE *)
+        apply Nat.eqb_eq in H. subst.
+        exists (word.or (word.slu (word.of_Z 1) (word.of_Z UART_STATUS_TXEMPTY_BIT))
+                        (word.slu (word.of_Z 1) (word.of_Z UART_STATUS_TXIDLE_BIT))).
+        exists IDLE.
+        split; [ solve_status_valid | left; reflexivity ].
+      }
+      { (* s = BUSY txlvl where txlvl <> 0 *)
+        exists (word.or (word.slu (word.of_Z 1) (word.of_Z UART_STATUS_TXEMPTY_BIT))
+                        (word.slu (word.of_Z 1) (word.of_Z UART_STATUS_TXIDLE_BIT))).
+        exists IDLE.
+        split; [ solve_status_valid | left; reflexivity ].
       }
     }
   Qed.
@@ -112,14 +126,64 @@ Section Proofs.
         | H1 : ?x = Some ?a, H2 : ?x = Some ?b |- _ =>
           rewrite H1 in H2; inversion H2; clear H2; subst
         | _ => idtac
+        end;
+    try lazymatch goal with
+    | H: [?a] = [?b] |- _ => inversion H; subst a
+    end.
+    all:try reflexivity.
+    all:cbv [status_matches_state] in *.
+
+    all:lazymatch goal with
+        | H0: _ \/ _, H1: _ \/ _ |- _ => destruct H0; destruct H1; logical_simplify; subst;
+            try reflexivity
+    end.
+    {
+      separate_flags.
+      lazymatch goal with
+      | H0: is_flag_set _ ?z = true, H1: negb (is_flag_set _ ?z) = true |- _ => rewrite H0 in H1;
+          discriminate
+      end.
+    }
+    {
+      destruct x.
+      {
+        simpl in *.
+        separate_flags.
+        lazymatch goal with
+        | H0: is_flag_set _ ?z = true, H1: negb (is_flag_set _ ?z) = true |- _ => rewrite H0 in H1;
+            discriminate
         end.
-    all:reflexivity.
+      }
+      {
+        simpl in *.
+        separate_flags.
+        lazymatch goal with
+        | H0: is_flag_set _ ?z = true, H1: negb (is_flag_set _ ?z) = true |- _ => rewrite H0 in H1;
+            discriminate
+        end.
+      }
+    }
+    {
+      lazymatch goal with
+      | H: S _ = S _ |- _ => apply Nat.succ_inj in H; subst
+      end.
+      reflexivity.
+    }
   Qed.
 
   Lemma reg_is_status :
     forall r,
     reg_addr r = word.of_Z (TOP_EARLGREY_UART0_BASE_ADDR + UART_STATUS_REG_OFFSET) ->
     r = STATUS.
+  Proof.
+    intros.
+    destruct r; apply reg_addr_unique; eauto.
+  Qed.
+
+  Lemma reg_is_wdata :
+    forall r,
+    reg_addr r = word.of_Z (TOP_EARLGREY_UART0_BASE_ADDR + UART_WDATA_REG_OFFSET) ->
+    r = WDATA.
   Proof.
     intros.
     destruct r; apply reg_addr_unique; eauto.
@@ -142,9 +206,75 @@ Section Proofs.
     lazymatch goal with
     | H: reg_addr _ = word.of_Z (base + UART_STATUS_REG_OFFSET) |- _ => apply reg_is_status in H; subst
     | H: reg_addr _ = word.of_Z (base + UART_CTRL_REG_OFFSET) |- _ => apply reg_is_ctrl in H; subst
+    | H: reg_addr _ = word.of_Z (base + UART_WDATA_REG_OFFSET) |- _ => apply reg_is_wdata in H; subst
     end.
 
+
   (***** Proofs for specific functions *****)
+  Global Instance spec_of_uart_tx_full : spec_of "b2_uart_tx_full" :=
+    fun function_env =>
+      forall (tr : trace) (m : mem) (R : _ -> Prop) (s : state),
+      (* no special requirements of the memory *)
+      R m ->
+      (* no constraints on current state *)
+      execution tr s ->
+      call function_env uart_tx_full tr m []
+        (fun tr' m' rets =>
+          exists (status out : word) (s' : state),
+            (* the new state matches the new trace *)
+            execution tr' s'
+            (* ...and there exists a single valid status-read step between
+               the old and new state, and the read result was [status] *)
+            /\ read_step s STATUS status s'
+            (* ...and all the same properties as before hold on the memory *)
+            /\ R m'
+            (* ...and there is one output value *)
+            /\ rets = [out]
+            (* ...and the output value is one if and only if the
+               txfull flag is set *)
+            /\ word.eqb out (word.of_Z 0)
+              = negb (is_flag_set status UART_STATUS_TXFULL_BIT)).
+  Lemma uart_tx_full_correct :
+    program_logic_goal_for_function! uart_tx_full.
+  Proof.
+    (* TODO the proof is almost identical to one for uart_tx_idle_correct, but
+       it is hard to generalize the proof becausae it calls the function twice *)
+    repeat straightline.
+    pose proof status_read_always_ok s as Hstat.
+    destruct Hstat as (x & s' & Hstat).
+    straightline_call; ssplit.
+    { instantiate (1 := STATUS). apply word.ring_morph_add. }
+    { cbv [state_machine.read_step uart_state_machine read_step] in *. eauto. }
+    { eauto. }
+    { repeat straightline.
+      straightline_call; eauto.
+      repeat straightline.
+      (* keep "execution a x" for later eassumption *)
+      lazymatch goal with
+      | H0 : execution tr _, H1: execution ?a _ |-  context [?tr] => rename H0 into Hexec; rename H1 into Hexec'
+      end.
+      pose proof Hexec' as HH.
+      simpl in Hexec'.
+      destruct Hexec' as (x' & Hexec').
+      destruct Hexec'.
+      replace s with x' in *.
+      2:{ eapply execution_unique; eauto. }
+      lazymatch goal with
+      | H: step _ _ _ _ _ |- _ => unfold step in H; simpl in H
+      end.
+      logical_simplify.
+      infer_reg_using_addr.
+      do 3 eexists; ssplit; eauto.
+      lazymatch goal with
+      | H: [_] = [_] |- _ => inversion H; subst
+      end.
+      unfold UART_STATUS_TXFULL_BIT in *.
+      apply is_flag_set_and_select_bits.
+      + cbv. reflexivity.
+      + split; try lia.
+    }
+  Qed.
+
 
   Global Instance spec_of_uart_tx_idle : spec_of "b2_uart_tx_idle" :=
     fun function_env =>
@@ -172,6 +302,8 @@ Section Proofs.
   Lemma uart_tx_idle_correct :
     program_logic_goal_for_function! uart_tx_idle.
   Proof.
+    (* TODO the proof is almost identical to one for uart_tx_idle_correct, but
+       it is hard to generalize the proof becausae it calls the function twice *)
     repeat straightline.
     pose proof status_read_always_ok s as Hstat.
     destruct Hstat as (x & s' & Hstat).
@@ -205,4 +337,224 @@ Section Proofs.
       apply is_flag_set_and_select_bits; lia.
     }
   Qed.
+
+  Ltac execution_trace Hexec Hexec' Hstep :=
+    lazymatch Hexec with
+    | execution ?t0 ?s0 =>
+        lazymatch Hexec' with
+        | execution ?t1 ?s1 =>
+            lazymatch Hstep with
+            | read_step s0 _ _ s1 => cbv [execution] in Hexec
+            end
+        end
+    end.
+
+
+  Global Instance spec_of_uart_putchar : spec_of "b2_uart_putchar" :=
+    fun function_env =>
+      forall (tr : trace) (m : mem) (R : _ -> Prop) (s : state) byte,
+      R m ->
+      (* uart must be in IDLE state before putchar *)
+      execution tr IDLE ->
+      call function_env uart_putchar tr m [byte]
+        (fun tr' m' rets =>
+          exists (s' : state),
+            (* uart must be in IDLE state after putchar *)
+            execution tr' IDLE
+            /\ R m'
+            /\ rets = []).
+  Lemma uart_putchar_correct :
+    program_logic_goal_for_function! uart_putchar.
+  Proof.
+    repeat straightline.
+
+    (* 1st while loop; we know that the loop will iterate once b/c s = IDLE *)
+    eapply unroll_while with (iterations:=1%nat). cbn [repeat_logic_step].
+    eexists.
+    split; repeat straightline.
+    subst cond.
+    push_unsigned.
+    rewrite word.eqb_eq.
+    2:{ reflexivity. }
+    split; [ lia | ].
+
+    repeat straightline.
+    (* calling uart_tx_full *)
+    straightline_call; eauto; logical_simplify.
+    repeat straightline.
+
+    lazymatch goal with
+    | H: read_step _ _ _ _ |- _ =>
+        cbv [read_step] in H; logical_simplify
+    end.
+
+    lazymatch goal with
+    | H: status_matches_state _ _ = true |- _ =>
+        cbv [status_matches_state] in H; subst
+    end.
+
+    separate_flags.
+
+    lazymatch goal with
+        | H0 : _ = negb (is_flag_set _ UART_STATUS_TXFULL_BIT),
+          H1 : negb (is_flag_set _ UART_STATUS_TXFULL_BIT) = true  |- _ =>
+              rewrite H1 in H0; apply word.eqb_true in H0; subst
+        end.
+
+    split.
+    {
+      subst cond.
+      push_unsigned.
+
+      rewrite word.unsigned_eqb.
+      rewrite word.unsigned_of_Z_1.
+      rewrite word.unsigned_of_Z_0.
+      reflexivity.
+    }
+
+    repeat straightline.
+
+    (* call bitfield_field32_write *)
+    straightline_call; eauto; repeat straightline.
+    (* call abs_mmio_write32 *)
+    straightline_call.
+    {
+      instantiate (1 := WDATA).
+      rewrite <- word.ring_morph_add.
+      cbv [state_machine.reg_addr uart_state_machine].
+      unfold reg_addr. reflexivity. }
+    {
+      cbn [state_machine.write_step uart_state_machine].
+      split; [reflexivity | ].
+      instantiate (2 := IDLE).
+      unfold write_step; reflexivity. }
+    { eauto. }
+
+    repeat straightline.
+
+    lazymatch goal with
+    | H0 : execution tr _, H1: execution ?a _ |-  context [?tr] => rename H0 into Hexec; rename H1 into Hexec'; subst a
+    end.
+    pose proof Hexec' as HH.
+    simpl in Hexec'.
+    destruct Hexec' as (x' & Hexec').
+    destruct Hexec'.
+    replace x' with IDLE in *.
+    2:{ eapply execution_unique; eauto. }
+    lazymatch goal with
+    | H: step _ _ _ _ _ |- _ => unfold step in H; simpl in H
+    end.
+    logical_simplify.
+    infer_reg_using_addr.
+
+    lazymatch goal with
+    | H: write_step _ _ _ ?x |- _ =>
+        cbv [write_step] in H; subst x
+    end.
+
+    (* 2nd while loop *)
+    (* loop until tx becomes IDLE again *)
+    apply atleastonce_localsmap
+      with (v0:=ncycles_processing)
+           (lt:=lt)
+           (invariant:=
+             fun i tr m l =>
+               execution tr (BUSY i) /\ R m).
+    { apply lt_wf. }
+    { (* Henter: case in which the loop breaks immediately (cannot happen) *)
+      repeat straightline.
+      exfalso. (* proof by contradiction *)
+
+      subst cond.
+      subst br.
+      lazymatch goal with
+      | H: word.unsigned _ = 0 |- _ =>
+          rewrite word.unsigned_if in H;
+          rewrite word.eqb_eq in H;
+          rewrite word.unsigned_of_Z_1 in H;
+          congruence
+      end. }
+    { (* Hpre: prof that invariant holds at loop start *)
+      ssplit; eauto. }
+    { (* Hbody *)
+      repeat lazymatch goal with
+             | H: execution ?a ?b |- _ => try clear dependent b; try clear dependent a; clear H
+             end.
+      repeat straightline.
+      straightline_call; eauto.
+      repeat straightline.
+
+      cbv [read_step] in *.
+      eexists; repeat straightline.
+      {
+        eexists.
+        lazymatch goal with
+        | |- map.get ?l _ = _ /\ _=> subst l
+        end.
+        rewrite map.get_put_same.
+        ssplit; eauto.
+        repeat straightline. }
+      { (* continuation case -- invariant holds *)
+        match goal with H : _ |- _ => apply word.if_nonzero, word.eqb_true in H end.
+        subst.
+        (* break into two possible s' : IDLE and BUSY *)
+        lazymatch goal with H : _ \/ _ |- _ => destruct H end;
+        logical_simplify; subst.
+        { (* s' = IDLE (cannot happen, should have exitted) *)
+          exfalso.
+          lazymatch goal with
+          | H: status_matches_state _ _ = true |- _ =>
+              cbv [status_matches_state] in H; simpl in H
+          end.
+          separate_flags.
+
+          lazymatch goal with
+          | H: word.eqb _ _ = _,
+          Hflag: is_flag_set _ UART_STATUS_TXIDLE_BIT = true |- _ =>
+              rewrite word.eqb_eq in H; [ | reflexivity ]
+                  ; rewrite <- Bool.negb_false_iff in Hflag
+          end.
+
+          lazymatch goal with
+          | H0: negb (is_flag_set _ UART_STATUS_TXIDLE_BIT) = _,
+            H1: true = negb (is_flag_set _ UART_STATUS_TXIDLE_BIT) |- _ =>
+                rewrite <- H1 in H0
+          end.
+          congruence.
+        }
+        { (* s' = BUSY v' *)
+          eexists.
+          repeat straightline; ssplit; eauto.
+        }
+      }
+      { (* break case -- postcondition holds *)
+        (* break into two possible s' cases : IDLE and BUSY *)
+        lazymatch goal with H : _ \/ _ |- _ => destruct H end;
+        logical_simplify; subst.
+        { (* s' = IDLE *)
+          eexists; ssplit; eauto. }
+        { (* s' = BUSY v' (cannot happen, should have continued) *)
+          exfalso.
+          cbv [status_matches_state] in *.
+
+          separate_flags.
+
+          autorewrite with push_unsigned in *.
+
+          lazymatch goal with
+          | H0: negb (is_flag_set _ UART_STATUS_TXIDLE_BIT) = _,
+            H1: word.eqb _ _ = negb (is_flag_set _ UART_STATUS_TXIDLE_BIT) |- _ =>
+                  rewrite <- H1 in H0;
+                  apply word.eqb_true in H0; subst
+          end.
+
+          lazymatch goal with
+          | H: (if _ then _ else _) = 0 |- _ => rewrite word.eqb_eq in H; [ | reflexivity ]
+          end.
+          congruence.
+        }
+      }
+    }
+  Qed.
+
 End Proofs.
